add values, merge defs with env, add lambdas support

LocalLang/AST.lean
@@ -5,21 +5,25 @@ inductive BinOp where
   | add
   | mul
 
+mutual
+inductive Value where
+  | nat (n : ℕ)
+  | closure (ps : List String) (body : Expr)
+
 inductive Expr where
+  | value (v : Value)
   | const (n : ℕ)
   | var (name : String)
   | binOp (op : BinOp) (e₁ e₂ : Expr)
   | letIn (name : String) (e₁ e₂ : Expr)
-  | funCall (f : String) (es : List Expr)
+  | funCall (e : Expr) (es : List Expr)
+end
 
-structure Func where
-  parameters : List String
-  body : Expr
+instance : OfNat Value n where
+  ofNat := .nat n
 
-abbrev Definitions := Std.HashMap String Func
+abbrev Env := Std.HashMap String Value
 
 structure Program where
-  definitions : Definitions
+  env : Env
   main : Expr
-
-abbrev Env := Std.HashMap String ℕ
