LocalLang/Ctx.lean
@@ -6,20 +6,23 @@ inductive Ctx : Type where
   | binOpRhs : ℕ → BinOp → Ctx → Ctx
   | letInExpr : String → Ctx → Expr → Ctx
   | letInBody : String → ℕ → Ctx → Ctx
+  | funCallBody : Ctx → List Expr → Ctx
 
 @[reducible] def Ctx.fill (e : Expr) : Ctx → Expr
   | hole => e
   | binOpLhs ctx op e' => Expr.binOp op (ctx.fill e) e'
-  | binOpRhs n op ctx => Expr.binOp op (.const n) (ctx.fill e)
+  | binOpRhs n op ctx => Expr.binOp op (.value (.nat n)) (ctx.fill e)
   | letInExpr x ctx e' => .letIn x (ctx.fill e) e'
-  | letInBody x n ctx => .letIn x (.const n) (ctx.fill e)
+  | letInBody x n ctx => .letIn x (.value (.nat n)) (ctx.fill e)
+  | funCallBody ctx es => .funCall (ctx.fill e) es
 
 @[reducible] def Ctx.updateEnv (env : Env) : Ctx → Env
   | hole => env
   | binOpLhs ctx _ _ => ctx.updateEnv env
   | binOpRhs _ _ ctx => ctx.updateEnv env
   | letInExpr _ ctx _ => ctx.updateEnv env
-  | letInBody x n ctx => ctx.updateEnv (env.insert x n)
+  | letInBody x n ctx => ctx.updateEnv (env.insert x (.nat n))
+  | funCallBody ctx _ => ctx.updateEnv env
 
 @[reducible] def Ctx.fillWithCtx (ctx : Ctx) (innerCtx : Ctx) : Ctx := match ctx with
   | .hole => innerCtx
@@ -27,3 +30,4 @@ inductive Ctx : Type where
   | .binOpRhs n op ctx₀ => .binOpRhs n op (Ctx.fillWithCtx ctx₀ innerCtx)
   | .letInExpr x ctx₀ e => .letInExpr x (Ctx.fillWithCtx ctx₀ innerCtx) e
   | .letInBody x n ctx₀ => .letInBody x n (Ctx.fillWithCtx ctx₀ innerCtx)
+  | .funCallBody ctx₀ es => .funCallBody (Ctx.fillWithCtx ctx₀ innerCtx) es
