LocalLang/Typing.lean
@@ -4,26 +4,31 @@ import LocalLang.Types
 -- in context Γ expression ε has Type T
 
 mutual
-  inductive TypeJdg : TypeContext → Expr → LLType → Prop where
-    | jdg_var {Γ : TypeContext}  {name : String} {ty : LLType} (H : Γ[name]? = some ty)
-                      : TypeJdg Γ (.var name) ty
-    | jdg_const {Γ : TypeContext} {n : ℕ} : TypeJdg Γ (.const n) LLType.nat
-    | jdg_fun {f} {Γ : TypeContext} {es : List Expr} {arg_types : List LLType} {T_return : LLType}
-                  (H_f : Γ[f]? = some (.func arg_types T_return))
-                  (H_args : TypeJdgList Γ es arg_types)
-                        : TypeJdg Γ (.funCall f es) (LLType.func arg_types T_return)
+  inductive Value.TypeJdg : Value → LLType → Prop where
+    | jdg_nat : Value.TypeJdg (.nat n) .nat
+    | jdg_closure {ps bd argTs retTy} : Expr.TypeJdg (.ofList (ps.zip argTs)) bd retTy
+      → Value.TypeJdg (.closure ps bd) (.func argTs retTy)
+
+  inductive Expr.TypeJdg : TypeContext → Expr → LLType → Prop where
+    | jdg_value {ty} : Value.TypeJdg v ty → Expr.TypeJdg Γ (.value v) ty
+    | jdg_var {Γ : TypeContext} {name : String} {ty : LLType} (H : Γ[name]? = some ty)
+                      : Expr.TypeJdg Γ (.var name) ty
+    | jdg_const {Γ : TypeContext} {n : ℕ} : Expr.TypeJdg Γ (.const n) LLType.nat
+    | jdg_fun {Γ : TypeContext} {es : List Expr} {arg_types : List LLType} {T_return : LLType}
+                  (f_jdg : Expr.TypeJdg Γ f (.func arg_types T_return))
+                  (H_args : Expr.TypeJdgList Γ es arg_types)
+                        : Expr.TypeJdg Γ (.funCall f es) (LLType.func arg_types T_return)
     | jdg_binOp {Γ : TypeContext} {op : BinOp} {e₁ e₂ : Expr}
-                (H₁ : TypeJdg Γ e₁ LLType.nat) (H₂ : TypeJdg Γ e₂ LLType.nat)
-                        : TypeJdg Γ (.binOp op e₁ e₂) .nat
+                (H₁ : Expr.TypeJdg Γ e₁ LLType.nat) (H₂ : Expr.TypeJdg Γ e₂ LLType.nat)
+                        : Expr.TypeJdg Γ (.binOp op e₁ e₂) .nat
     | jdg_let_in {Γ : TypeContext} {name : String} {e₁ e₂ : Expr} {ty₁ ty₂ : LLType}
-                (H₁ : TypeJdg Γ e₁ ty₁)
-                (H₂ : TypeJdg (Γ.insert name ty₁) e₂ ty₂)
-                        : TypeJdg  Γ (.letIn name e₁ e₂) ty₂
+                (H₁ : Expr.TypeJdg Γ e₁ ty₁)
+                (H₂ : Expr.TypeJdg (Γ.insert name ty₁) e₂ ty₂)
+                        : Expr.TypeJdg  Γ (.letIn name e₁ e₂) ty₂
 
-
-  inductive TypeJdgList : TypeContext -> List Expr -> List LLType -> Prop
-    | nil : TypeJdgList Γ [] []
+  inductive Expr.TypeJdgList : TypeContext -> List Expr -> List LLType -> Prop
+    | nil : Expr.TypeJdgList Γ [] []
     | cons {e : Expr} {T : LLType} {es : List Expr} {Ts : List LLType}
-          (h_e : TypeJdg Γ e T) (h_es : TypeJdgList Γ es Ts)
-          : TypeJdgList Γ (e :: es) (T :: Ts)
+          (h_e : Expr.TypeJdg Γ e T) (h_es : Expr.TypeJdgList Γ es Ts)
+          : Expr.TypeJdgList Γ (e :: es) (T :: Ts)
 end
