LocalLang/TypingExamples.lean
@@ -1,16 +1,3 @@
 import LocalLang.Typing
 
 -- Examples for TypeJdg
-example : TypeJdg {} (.const 5) .nat := by
-  apply TypeJdg.jdg_const
-
-example : TypeJdg {("x", .nat)} (.var "x") .nat := by
-  apply TypeJdg.jdg_var
-  simp
-
-def ctx : TypeContext := {("add", .func [.nat] .nat), ("x", .nat)}
-
-example : TypeJdg ctx (.funCall "add" [.var "x"]) (LLType.func [.nat] .nat) := by
-  apply TypeJdg.jdg_fun
-  · simp [ctx]
-  · sorry
