LocalLang/EvaluatorTests.lean
@@ -1,14 +1,1 @@
 import LocalLang.Evaluator
-
--- test for updateEnv, ensures that existing values get overwritten correctly
-example :=
-  let V : Env := .ofList [("x", 1)]
-  let func : Func := ⟨["x"], .const 0⟩
-  let V' := func.updateEnv V [2]
-  let result : V'["x"]? = some 2 := by
-    unfold V'
-    unfold V
-    rw [Func.updateEnv, List.zip, List.zipWith, ← Std.HashMap.get?_eq_getElem?,
-      Std.HashMap.get?_union]
-    simp
-  result
