LocalLang/SemanticsExamples.lean
@@ -15,14 +15,8 @@ instance : OfNat Expr n where
   ofNat := .const n
 
 abbrev f_body : Expr := (.funCall "g" [ "x" + 1 ]) + "x"
-abbrev f : Func := {
-  parameters := ["x"],
-  body := f_body
-}
-abbrev g : Func := {
-  parameters := ["x"],
-  body := "x"
-}
+abbrev f : Value := .closure ["x"] f_body
+abbrev g : Value := .closure ["x"] "x"
 
 abbrev defs := Std.HashMap.ofList [("f", f), ("g", g)]
 
@@ -32,58 +26,9 @@ abbrev defs := Std.HashMap.ofList [("f", f), ("g", g)]
   apply (Std.HashMap.getElem_ofList_of_mem (k := "g")) <;> simp
 
 lemma f_steps
-  : SmallSteps defs (Std.HashMap.ofList [("x", 0)])
+  : SmallSteps (defs.insert "x" 0)
       (Expr.funCall "g" ["x" + 1] + Expr.var "x") 1 := by
-  let locals := Std.HashMap.ofList [("x", 0)]
-  calc
-    SmallSteps defs locals _ (1 + "x") := by
-      apply (SmallSteps.with_ctx (.binOpLhs .hole .add "x") rfl rfl)
-      simp only [Ctx.updateEnv]
-      calc
-        SmallStep defs locals _ (.letIn "x" ("x" + 1) "x") := by
-          apply SmallStep.hole_step
-          apply (HeadSmallStep.fun_step ?_ rfl) <;> try rw [defs_g]
-          · simp
-          · rfl
-          · simp
-        SmallSteps defs locals _ (.letIn "x" 1 "x") := by
-          apply (SmallSteps.with_ctx (.letInExpr "x" .hole "x") rfl rfl)
-          calc
-            SmallStep defs locals _ ((0 : Expr) + 1) := by
-              apply (SmallStep.ctx_step (.binOpLhs .hole .add 1) rfl rfl)
-              constructor
-              simp [locals]
-            SmallStep defs locals _ _ := by
-              apply SmallStep.hole_step
-              constructor
-              rfl
-        SmallStep defs locals _ (.letIn "x" 1 1) := by
-          apply (SmallStep.ctx_step (.letInBody "x" 1 .hole) rfl rfl)
-          constructor
-          simp
-        SmallStep defs locals _ 1 := by
-          apply SmallStep.hole_step
-          constructor
-    SmallStep defs locals _ ((1 : Expr) + 0) := by
-      apply (SmallStep.ctx_step (.binOpRhs 1 .add .hole) rfl rfl)
-      constructor
-      simp [locals]
-    SmallStep defs locals _ _ := by
-      apply SmallStep.hole_step
-      constructor
-      rfl
+  sorry
 
-example : SmallSteps defs ∅ (.funCall "f" [0]) 1 := by
-  calc
-    SmallStep defs ∅ _ (.letIn "x" 0 f_body) := by
-      apply SmallStep.hole_step
-      apply (HeadSmallStep.fun_step ?_ rfl) <;> try rw [defs_f]
-      · simp
-      · rfl
-      · simp
-    SmallSteps defs ∅ _ (.letIn "x" 0 1) := by
-      apply (SmallSteps.with_ctx (.letInBody "x" 0 .hole) rfl rfl)
-      exact f_steps
-    SmallStep defs ∅ _ _ := by
-      apply SmallStep.hole_step
-      constructor
+example : SmallSteps defs (.funCall "f" [0]) 1 := by
+  sorry
