LocalLang/TypingGuarantees.lean
@@ -3,35 +3,13 @@ import LocalLang.Semantics
 import LocalLang.Types
 import LocalLang.Typing
 
-def EnvRespectsCtx (Γ : TypeContext) (V : Env) : Prop :=
-  ∀ (x : String) (n : ℕ), V[x]? = some n → Γ[x]? = LLType.nat
+def EnvRespectsCtx (Γ : TypeContext) (V : Env) : Prop := sorry
 
 -- TODO: prove
 -- TODO: V and Γ should be related
-theorem preservation (Γ : TypeContext) (e e' : Expr) (ty : LLType) (defs : Definitions)
+theorem preservation (Γ : TypeContext) (e e' : Expr) (ty : LLType)
     (h_env_respects : EnvRespectsCtx Γ V)
-  : TypeJdg Γ e ty → HeadSmallStep defs V e e' → TypeJdg Γ e' ty := by
-  intro h_jdg b
-  induction b
-  · cases h_jdg
-    · rename_i x n a relΓ
-      unfold EnvRespectsCtx at h_env_respects
-      let ent_ctx_link := h_env_respects x n a
-      let symmRelΓ := relΓ.symm
-      have ty_eq := Option.some.inj (symmRelΓ.trans ent_ctx_link)
-      rw [ty_eq]
-      constructor
-  · cases h_jdg
-    · rename_i H₁ H₂
-      apply TypeJdg.jdg_const
-  · rename_i name val n
-    cases h_jdg
-    · rename_i H₁ H₂
-      cases H₂
-      constructor
-  · cases h_jdg
-    rename_i f es arg_types T_return h_f h_args
-    sorry
+  : Expr.TypeJdg Γ e ty → HeadSmallStep V e e' → Expr.TypeJdg Γ e' ty := sorry
 
 -- Progress: if TypeJdg Γ e ty, then e can take a step.
 -- TODO: formalize
